verified/ARMprint.dfy
@@ -1,3 +1,115 @@
 include "ARMdef.dfy"
 
-function method sp_CNil():codes { CNil }
+method cma()       { print(", "); }
+method nl()        { print("\n"); }
+method not_impl()  { print("  !!!NOT IMPLEMENTED!!!"); }
+
+function method cmpNot(c:ocmp):ocmp
+{
+  match c
+    case OEq => ONe
+    case ONe => OEq
+    case OLe => OGt
+    case OGe => OLt
+    case OLt => OGe
+    case OGt => OLe
+}
+
+method printBcc(c:ocmp)
+{
+	match c
+	{
+		case OEq => print("B EQ");
+		case ONe => print("B NE ");
+		case OLe => print("B LE ");
+		case OGe => print("B GE ");
+		case OLt => print("B LT ");
+		case OGt => print("B GT ");
+	}
+}
+
+method printId(id:id)
+{
+	match id
+	{
+		case IdARMReg(r) => { match r
+			case R(i) => print("r"); print(i); }
+    	case IdGlobal(g) => print(" !!!NOT IMPLEMENTED!!!");
+    	case IdLocal(l) => print(" !!!NOT IMPLEMENTED!!!");
+    	case IdStackSlot(i) => print(" !!! NOT IMPLEMENTED!!!");
+	}
+}
+
+method printOperand(o:operand)
+{
+  match o
+  {
+    case OConst(n) =>
+    {
+      if 0 <= n < 0x1_0000_0000 { print(n); }
+      else { print(" !!!NOT IMPLEMENTED!!!"); }
+    }
+    case OVar(x) => printId(x);
+    case OHeap(addr) => print(" !!!NOT IMPLEMENTED!!!");
+  }
+}
+
+method printIns(ins:ins)
+{
+	match ins
+	{
+		case ADD(dest, src1, src2) =>
+			print("  Add"); printOperand(dest); cma();
+				printOperand(src1); cma();
+				printOperand(src2); nl();
+	}
+}
+
+method printBlock(b:codes, n:int) returns(n':int)
+{
+  n' := n;
+  var i := b;
+  while (i.sp_CCons?)
+    decreases i
+  {
+    n' := printCode(i.hd, n');
+    i := i.tl;
+  }
+}
+
+method printCode(c:code, n:int) returns(n':int)
+{
+	match c
+	{
+		case Ins(ins) => printIns(ins); n':= n;
+    	case Block(block) => n' := printBlock(block, n);
+		case IfElse(ifb, ift, iff) => {
+			var false_branch := n;
+			var end_of_block := n + 1;
+			// Do comparison
+			print("  cmp "); printOperand(ifb.o1); cma();
+				printOperand(ifb.o2); nl();
+			// Branch to false branch if cond is false
+			printBcc(cmpNot(ifb.cmp)); print("L"); print(false_branch); nl();
+			// True branch
+      		n' := printCode(ift, n + 2);
+      		print("  B L"); print(end_of_block); nl(); 
+      		print("L"); print(false_branch); print(":\n");
+			// False branch
+      		n' := printCode(iff, n');
+			// Label end of block
+      		print("L"); print(end_of_block); print(":\n");
+		}	
+    	case While(b, loop) =>
+    	{
+    	  var n1 := n;
+    	  var n2 := n + 1;
+    	  print("  B L"); print(n2); print("\n");
+    	  print("L"); print(n1); print(":\n");
+    	  n' := printCode(loop, n + 2);
+    	  print("L"); print(n2); print(":\n");
+    	  print("  cmp "); printOperand(b.o1); print(", "); printOperand(b.o2); print("\n");
+    	  printBcc(cmpNot(b.cmp)); print("L"); print(n1); print("\n");
+    	}
+	}
+}
